src/3d/prelude/EverParse3d.InputBuffer.fst
@@ -7,30 +7,49 @@ module U32 = FStar.UInt32
 module LPL = LowParse.Low.Base
 module R = EverParse3d.Readable
 module G = FStar.Ghost
-module Aux = EverParse3d.InputBuffer.Aux
 
 open LowParse.Low.Base
 
-let input_buffer_t = Aux.input_buffer
+inline_for_extraction
+noextract
+let base_t (len: U32.t)
+= (base: B.buffer LPL.byte { U32.v len <= B.length base })
+
+inline_for_extraction
+noextract
+noeq
+type input_buffer_perm (len: U32.t) = 
+{
+  p_base: Ghost.erased (base_t len);
+  p_perm: R.perm p_base;
+}
+
+let input_buffer_t len =
+  (p: (base_t len & input_buffer_perm len) { Ghost.reveal (snd p).p_base == fst p })
 
 let slice_of #len x =
-  { LPL.base = dfst x; LPL.len = len }
+  { LPL.base = fst x; LPL.len = len }
 
-let perm_of x = dsnd x
+let perm_of x = (snd x).p_perm
 
 let truncate_input_buffer #len0 x len =
   match x with
-  | (| base, perm |) -> (| base, perm |)
+  | (base, perm) ->
+    [@inline_let]
+    let base' : base_t len = base in
+    [@inline_let]
+    let perm' : R.perm base' = perm.p_perm in
+    (base, ({ p_base = base'; p_perm = perm' }))
 
 let drop sl from to =
   match sl with
-  | (| base, perm |) ->
-    R.drop perm from to
+  | (base, perm) ->
+    R.drop (perm.p_perm <: R.perm base) from to
 
 (* TODO: remove the slice here *)
 let read_with_perm #k #t #p r j #len sl pos =
   match sl with
-  | (| base, _ |) ->
+  | (base, _) ->
   [@inline_let] let sl' : LPL.slice triv triv = { LPL.base = base; LPL.len = len } in
   let pos' = j sl' pos in
   drop sl pos pos' ;
@@ -40,5 +59,5 @@ let puint8 = B.buffer LPL.byte
 
 let offset sl off =
   match sl with
-  | (| base, _ |) ->
+  | (base, _) ->
   B.moffset triv base off
